src/CPSA/Roletran/Derivation.hs
@@ -42,7 +42,7 @@ derive r =
     -- Construct the statements from the inputs
     preamble <- deriveInputs r fresh (reverse bindings)
     -- Construct a list of the return types.
-    let outs = map sort (routputs r)
+    let outs = map kind (routputs r)
     -- Construct the statements that form the body of the procedure.
     stmts <- deriveStmts r preamble
     return $ mkProc
@@ -59,7 +59,7 @@ bindInputs ts =
   foldl f (0, [], []) ts
   where
     f (fresh, binding, ins) t =
-      (fresh + 1, (t, fresh) : binding, (fresh, sort t) : ins)
+      (fresh + 1, (t, fresh) : binding, (fresh, kind t) : ins)
 
 -- The state association with compilation
 type State = (Vari, CompStore, [Stmt])
@@ -115,7 +115,7 @@ deriveEvent uniques st ((Out pos ch t), i) =
     return (
       freshVar st,
       compStore st,
-      Send chan (v, sort t) : statements st)
+      Send chan (v, kind t) : statements st)
 -- Compile a recv event.
 deriveEvent _ st ((In pos ch t), _) =
   case receivable t of
@@ -124,7 +124,7 @@ deriveEvent _ st ((In pos ch t), _) =
         -- Synthesize the channel.
         (st, chan) <- build pos (recvCmt pos st) ch
         let (fresh, cs, stmts) = st
-        let recv = Recv (fresh, sort t) chan
+        let recv = Recv (fresh, kind t) chan
         let st' = (fresh + 1, cs, recv : stmts)
         -- Associate fresh with the received message.
         reduce pos st' [(t, fresh)]
@@ -149,7 +149,7 @@ deriveUniques uniques i st =
     f st@(fresh, cs, stmts) (t, j)
       | i == j = (fresh + 1,
                   M.insert t fresh cs, -- Bind fresh to a nonce.
-                  Bind (fresh, sort t) (Nonce (sort t)) : stmts)
+                  Bind (fresh, kind t) (Nonce (kind t)) : stmts)
       | otherwise = st
 
 -- Synthesize a term and fail when it can't be built.
@@ -180,7 +180,7 @@ synthPair st t x y =
     return (
       (fresh + 1,
        M.insert t fresh cs,     -- Bind fresh to the pair t.
-       Bind (fresh, Mesg) (Pair (v, sort x) (u, sort y)) : stmts),
+       Bind (fresh, kind t) (Pair (v, kind x) (u, kind y)) : stmts),
       fresh)
 
 synthEncr :: State -> Term -> Term -> Term -> Maybe (State, Vari)
@@ -191,7 +191,7 @@ synthEncr st t x y =
     return (
       (fresh + 1,
        M.insert t fresh cs,     -- Bind fresh to the encryption t.
-       Bind (fresh, Mesg) (Encr (v, sort x) (u, sort y)) : stmts),
+       Bind (fresh, kind t) (Encr (v, kind x) (u, kind y)) : stmts),
       fresh)
 
 synthHash :: State -> Term -> Term -> Maybe (State, Vari)
@@ -201,7 +201,7 @@ synthHash st t x  =
     return (
       (fresh + 1,
        M.insert t fresh cs,     -- Bind fresh to the hash t.
-       Bind (fresh, Mesg) (Hash (v, sort x)) : stmts),
+       Bind (fresh, kind t) (Hash (v, kind x)) : stmts),
       fresh)
 
 synthTag :: State -> Term -> String -> Maybe (State, Vari)
@@ -209,7 +209,7 @@ synthTag (fresh, cs, stmts) t s  =
   return (
     (fresh + 1,
      M.insert t fresh cs,       -- Bind fresh to the tag.
-     Bind (fresh, Mesg) (Tagg s) : stmts),
+     Bind (fresh, kind t) (Tagg s) : stmts),
     fresh)
 
 -- Reduce a received term.  This is by far the trickiest code.  The
@@ -246,8 +246,8 @@ loopPair :: MonadFail m => Pos -> State ->
             Term -> Vari -> Term -> Term -> m State
 loopPair pos (fresh, cs, stmts) recvd todo t v x y =
   do
-    let stmtX = Bind (fresh, sort x) (Frst (sort x) v)
-    let stmtY = Bind (fresh + 1, sort y) (Scnd (sort y) v)
+    let stmtX = Bind (fresh, kind x) (Frst (kind x) v)
+    let stmtY = Bind (fresh + 1, kind y) (Scnd (kind y) v)
     let st = (
           fresh + 2,
           M.insert t v cs,      -- Add pair to the compile time store
@@ -266,7 +266,7 @@ loopEncr pos st more recvd todo t v x y =
       loop pos st more recvd ((t, v) : todo)
     Just ((fresh, cs, stmts), k) ->
       do
-        let stmt = Bind (fresh, sort x) (Decr (sort x) v (k, sort y))
+        let stmt = Bind (fresh, kind x) (Decr (kind x) v (k, kind y))
         let st = (
               fresh + 1,
               M.insert t v cs, -- Add encryption to the compile time store
@@ -282,7 +282,7 @@ loopHash pos st more recvd todo t v =
       loop pos st more recvd ((t, v) : todo)
     Just ((fresh, cs, stmts), h) ->
       do
-        let stmt = Same (sort t) v h
+        let stmt = Same (kind t) v h
         let st = (fresh, cs, stmt : stmts)
         loop pos st True recvd todo
 
@@ -296,7 +296,7 @@ loopOther pos st@(fresh, cs, stmts) more recvd todo t v =
       loop pos (fresh, M.insert t v cs, stmts) True recvd todo
     Just ((fresh, cs, stmts), h) ->
       do                        -- Otherwise, check sameness
-        let stmt = Same (sort t) v h
+        let stmt = Same (kind t) v h
         let st = (fresh, cs, stmt : stmts)
         loop pos st more recvd todo
 
