coq/Examples/Nsl.v
@@ -12,21 +12,21 @@ Definition init: proc :=
   [(0, Chan); (1, Ikey); (2, Akey); (3, Akey)]
   [
    (* Send (nsl.scm:7:6) *)
-   Bind (4, Text) (Nonce);
-   Bind (5, Mesg) (Pair 4 2);
-   Bind (6, Mesg) (Encr 5 3);
+   Bind (4, Text) (Nonce_);
+   Bind (5, Pair) (Pair_ 4 2);
+   Bind (6, Aenc) (Encr_ 5 3);
    Send 0 6;
    (* Recv (nsl.scm:8:6) *)
-   Bind (7, Mesg) (Recv 0);
-   Bind (8, Mesg) (Decr 7 1);
-   Bind (9, Text) (Frst 8);
-   Bind (10, Mesg) (Scnd 8);
+   Bind (7, Aenc) (Recv_ 0);
+   Bind (8, Pair) (Decr_ 7 1);
+   Bind (9, Text) (Frst_ 8);
+   Bind (10, Pair) (Scnd_ 8);
    Same 9 4;
-   Bind (11, Text) (Frst 10);
-   Bind (12, Akey) (Scnd 10);
+   Bind (11, Text) (Frst_ 10);
+   Bind (12, Akey) (Scnd_ 10);
    Same 12 3;
    (* Send (nsl.scm:9:6) *)
-   Bind (13, Mesg) (Encr 11 3);
+   Bind (13, Aenc) (Encr_ 11 3);
    Send 0 13;
    Return [4; 11]
   ].
@@ -38,20 +38,20 @@ Definition resp: proc :=
   [(0, Chan); (1, Ikey); (2, Akey); (3, Akey)]
   [
    (* Recv (nsl.scm:16:6) *)
-   Bind (4, Mesg) (Recv 0);
-   Bind (5, Mesg) (Decr 4 1);
-   Bind (6, Text) (Frst 5);
-   Bind (7, Akey) (Scnd 5);
+   Bind (4, Aenc) (Recv_ 0);
+   Bind (5, Pair) (Decr_ 4 1);
+   Bind (6, Text) (Frst_ 5);
+   Bind (7, Akey) (Scnd_ 5);
    Same 7 3;
    (* Send (nsl.scm:17:6) *)
-   Bind (8, Text) (Nonce);
-   Bind (9, Mesg) (Pair 8 2);
-   Bind (10, Mesg) (Pair 6 9);
-   Bind (11, Mesg) (Encr 10 3);
+   Bind (8, Text) (Nonce_);
+   Bind (9, Pair) (Pair_ 8 2);
+   Bind (10, Pair) (Pair_ 6 9);
+   Bind (11, Aenc) (Encr_ 10 3);
    Send 0 11;
    (* Recv (nsl.scm:18:6) *)
-   Bind (12, Mesg) (Recv 0);
-   Bind (13, Text) (Decr 12 1);
+   Bind (12, Aenc) (Recv_ 0);
+   Bind (13, Text) (Decr_ 12 1);
    Same 13 8;
    Return [8; 6]
   ].
