coq/Examples/Otway_rees.v
@@ -12,21 +12,21 @@ Definition init: proc :=
   [(0, Chan); (1, Name); (2, Name); (3, Skey)]
   [
    (* Send (otway_rees.scm:12:6) *)
-   Bind (4, Text) (Nonce);
-   Bind (5, Mesg) (Pair 2 4);
-   Bind (6, Mesg) (Pair 1 5);
+   Bind (4, Text) (Nonce_);
+   Bind (5, Pair) (Pair_ 2 4);
+   Bind (6, Pair) (Pair_ 1 5);
    Send 0 6;
    (* Recv (otway_rees.scm:13:6) *)
-   Bind (7, Mesg) (Recv 0);
-   Bind (8, Mesg) (Decr 7 3);
-   Bind (9, Text) (Frst 8);
-   Bind (10, Mesg) (Scnd 8);
+   Bind (7, Senc) (Recv_ 0);
+   Bind (8, Pair) (Decr_ 7 3);
+   Bind (9, Text) (Frst_ 8);
+   Bind (10, Pair) (Scnd_ 8);
    Same 9 4;
-   Bind (11, Name) (Frst 10);
-   Bind (12, Mesg) (Scnd 10);
+   Bind (11, Name) (Frst_ 10);
+   Bind (12, Pair) (Scnd_ 10);
    Same 11 1;
-   Bind (13, Name) (Frst 12);
-   Bind (14, Skey) (Scnd 12);
+   Bind (13, Name) (Frst_ 12);
+   Bind (14, Skey) (Scnd_ 12);
    Same 13 2;
    Return [14]
   ].
@@ -38,31 +38,31 @@ Definition resp: proc :=
   [(0, Chan); (1, Chan); (2, Name); (3, Skey)]
   [
    (* Recv (otway_rees.scm:24:6) *)
-   Bind (4, Mesg) (Recv 0);
-   Bind (5, Name) (Frst 4);
-   Bind (6, Mesg) (Scnd 4);
-   Bind (7, Name) (Frst 6);
-   Bind (8, Text) (Scnd 6);
+   Bind (4, Pair) (Recv_ 0);
+   Bind (5, Name) (Frst_ 4);
+   Bind (6, Pair) (Scnd_ 4);
+   Bind (7, Name) (Frst_ 6);
+   Bind (8, Text) (Scnd_ 6);
    Same 7 2;
    (* Send (otway_rees.scm:25:6) *)
-   Bind (9, Text) (Nonce);
-   Bind (10, Mesg) (Pair 8 9);
-   Bind (11, Mesg) (Pair 2 10);
-   Bind (12, Mesg) (Pair 5 11);
+   Bind (9, Text) (Nonce_);
+   Bind (10, Pair) (Pair_ 8 9);
+   Bind (11, Pair) (Pair_ 2 10);
+   Bind (12, Pair) (Pair_ 5 11);
    Send 1 12;
    (* Recv (otway_rees.scm:26:6) *)
-   Bind (13, Mesg) (Recv 1);
-   Bind (14, Mesg) (Frst 13);
-   Bind (15, Mesg) (Scnd 13);
-   Bind (16, Mesg) (Decr 15 3);
-   Bind (17, Text) (Frst 16);
-   Bind (18, Mesg) (Scnd 16);
+   Bind (13, Pair) (Recv_ 1);
+   Bind (14, Mesg) (Frst_ 13);
+   Bind (15, Senc) (Scnd_ 13);
+   Bind (16, Pair) (Decr_ 15 3);
+   Bind (17, Text) (Frst_ 16);
+   Bind (18, Pair) (Scnd_ 16);
    Same 17 9;
-   Bind (19, Name) (Frst 18);
-   Bind (20, Mesg) (Scnd 18);
+   Bind (19, Name) (Frst_ 18);
+   Bind (20, Pair) (Scnd_ 18);
    Same 19 5;
-   Bind (21, Name) (Frst 20);
-   Bind (22, Skey) (Scnd 20);
+   Bind (21, Name) (Frst_ 20);
+   Bind (22, Skey) (Scnd_ 20);
    Same 21 2;
    (* Send (otway_rees.scm:27:6) *)
    Send 0 14;
@@ -76,24 +76,24 @@ Definition serv: proc :=
   [(0, Chan); (1, Name); (2, Name); (3, Skey); (4, Skey)]
   [
    (* Recv (otway_rees.scm:37:6) *)
-   Bind (5, Mesg) (Recv 0);
-   Bind (6, Name) (Frst 5);
-   Bind (7, Mesg) (Scnd 5);
+   Bind (5, Pair) (Recv_ 0);
+   Bind (6, Name) (Frst_ 5);
+   Bind (7, Pair) (Scnd_ 5);
    Same 6 1;
-   Bind (8, Name) (Frst 7);
-   Bind (9, Mesg) (Scnd 7);
+   Bind (8, Name) (Frst_ 7);
+   Bind (9, Pair) (Scnd_ 7);
    Same 8 2;
-   Bind (10, Text) (Frst 9);
-   Bind (11, Text) (Scnd 9);
+   Bind (10, Text) (Frst_ 9);
+   Bind (11, Text) (Scnd_ 9);
    (* Send (otway_rees.scm:38:6) *)
-   Bind (12, Skey) (Nonce);
-   Bind (13, Mesg) (Pair 2 12);
-   Bind (14, Mesg) (Pair 1 13);
-   Bind (15, Mesg) (Pair 10 14);
-   Bind (16, Mesg) (Encr 15 3);
-   Bind (17, Mesg) (Pair 11 14);
-   Bind (18, Mesg) (Encr 17 4);
-   Bind (19, Mesg) (Pair 16 18);
+   Bind (12, Skey) (Nonce_);
+   Bind (13, Pair) (Pair_ 2 12);
+   Bind (14, Pair) (Pair_ 1 13);
+   Bind (15, Pair) (Pair_ 10 14);
+   Bind (16, Senc) (Encr_ 15 3);
+   Bind (17, Pair) (Pair_ 11 14);
+   Bind (18, Senc) (Encr_ 17 4);
+   Bind (19, Pair) (Pair_ 16 18);
    Send 0 19;
    Return [12]
   ].
