coq/Examples/Yahalom.v
@@ -12,25 +12,25 @@ Definition init: proc :=
   [(0, Chan); (1, Chan); (2, Name); (3, Name); (4, Skey)]
   [
    (* Send (yahalom.scm:13:6) *)
-   Bind (5, Text) (Nonce);
-   Bind (6, Mesg) (Pair 2 5);
+   Bind (5, Text) (Nonce_);
+   Bind (6, Pair) (Pair_ 2 5);
    Send 0 6;
    (* Recv (yahalom.scm:14:6) *)
-   Bind (7, Mesg) (Recv 1);
-   Bind (8, Mesg) (Frst 7);
-   Bind (9, Mesg) (Scnd 7);
-   Bind (10, Mesg) (Decr 8 4);
-   Bind (11, Name) (Frst 10);
-   Bind (12, Mesg) (Scnd 10);
+   Bind (7, Pair) (Recv_ 1);
+   Bind (8, Senc) (Frst_ 7);
+   Bind (9, Mesg) (Scnd_ 7);
+   Bind (10, Pair) (Decr_ 8 4);
+   Bind (11, Name) (Frst_ 10);
+   Bind (12, Pair) (Scnd_ 10);
    Same 11 3;
-   Bind (13, Skey) (Frst 12);
-   Bind (14, Mesg) (Scnd 12);
-   Bind (15, Text) (Frst 14);
-   Bind (16, Text) (Scnd 14);
+   Bind (13, Skey) (Frst_ 12);
+   Bind (14, Pair) (Scnd_ 12);
+   Bind (15, Text) (Frst_ 14);
+   Bind (16, Text) (Scnd_ 14);
    Same 15 5;
    (* Send (yahalom.scm:15:6) *)
-   Bind (17, Mesg) (Encr 16 13);
-   Bind (18, Mesg) (Pair 9 17);
+   Bind (17, Senc) (Encr_ 16 13);
+   Bind (18, Pair) (Pair_ 9 17);
    Send 0 18;
    Return [13]
   ].
@@ -42,25 +42,25 @@ Definition resp: proc :=
   [(0, Chan); (1, Chan); (2, Name); (3, Skey)]
   [
    (* Recv (yahalom.scm:26:6) *)
-   Bind (4, Mesg) (Recv 0);
-   Bind (5, Name) (Frst 4);
-   Bind (6, Text) (Scnd 4);
+   Bind (4, Pair) (Recv_ 0);
+   Bind (5, Name) (Frst_ 4);
+   Bind (6, Text) (Scnd_ 4);
    (* Send (yahalom.scm:27:6) *)
-   Bind (7, Text) (Nonce);
-   Bind (8, Mesg) (Pair 6 7);
-   Bind (9, Mesg) (Pair 5 8);
-   Bind (10, Mesg) (Encr 9 3);
-   Bind (11, Mesg) (Pair 2 10);
+   Bind (7, Text) (Nonce_);
+   Bind (8, Pair) (Pair_ 6 7);
+   Bind (9, Pair) (Pair_ 5 8);
+   Bind (10, Senc) (Encr_ 9 3);
+   Bind (11, Pair) (Pair_ 2 10);
    Send 1 11;
    (* Recv (yahalom.scm:28:6) *)
-   Bind (12, Mesg) (Recv 0);
-   Bind (13, Mesg) (Frst 12);
-   Bind (14, Mesg) (Scnd 12);
-   Bind (15, Mesg) (Decr 13 3);
-   Bind (16, Name) (Frst 15);
-   Bind (17, Skey) (Scnd 15);
+   Bind (12, Pair) (Recv_ 0);
+   Bind (13, Senc) (Frst_ 12);
+   Bind (14, Senc) (Scnd_ 12);
+   Bind (15, Pair) (Decr_ 13 3);
+   Bind (16, Name) (Frst_ 15);
+   Bind (17, Skey) (Scnd_ 15);
    Same 16 5;
-   Bind (18, Text) (Decr 14 17);
+   Bind (18, Text) (Decr_ 14 17);
    Same 18 7;
    Return [5; 17]
   ].
@@ -72,15 +72,15 @@ Definition serv_init: proc :=
   [(0, Chan); (1, Name); (2, Skey)]
   [
    (* Recv (yahalom.scm:39:6) *)
-   Bind (3, Mesg) (Recv 0);
-   Bind (4, Name) (Frst 3);
-   Bind (5, Mesg) (Scnd 3);
+   Bind (3, Pair) (Recv_ 0);
+   Bind (4, Name) (Frst_ 3);
+   Bind (5, Senc) (Scnd_ 3);
    Same 4 1;
-   Bind (6, Mesg) (Decr 5 2);
-   Bind (7, Name) (Frst 6);
-   Bind (8, Mesg) (Scnd 6);
-   Bind (9, Text) (Frst 8);
-   Bind (10, Text) (Scnd 8);
+   Bind (6, Pair) (Decr_ 5 2);
+   Bind (7, Name) (Frst_ 6);
+   Bind (8, Pair) (Scnd_ 6);
+   Bind (9, Text) (Frst_ 8);
+   Bind (10, Text) (Scnd_ 8);
    Return [7; 9; 10]
   ].
 
@@ -91,14 +91,14 @@ Definition serv_complete: proc :=
   [(0, Chan); (1, Name); (2, Name); (3, Skey); (4, Skey); (5, Text); (6, Text)]
   [
    (* Send (yahalom.scm:48:6) *)
-   Bind (7, Skey) (Nonce);
-   Bind (8, Mesg) (Pair 5 6);
-   Bind (9, Mesg) (Pair 7 8);
-   Bind (10, Mesg) (Pair 2 9);
-   Bind (11, Mesg) (Encr 10 3);
-   Bind (12, Mesg) (Pair 1 7);
-   Bind (13, Mesg) (Encr 12 4);
-   Bind (14, Mesg) (Pair 11 13);
+   Bind (7, Skey) (Nonce_);
+   Bind (8, Pair) (Pair_ 5 6);
+   Bind (9, Pair) (Pair_ 7 8);
+   Bind (10, Pair) (Pair_ 2 9);
+   Bind (11, Senc) (Encr_ 10 3);
+   Bind (12, Pair) (Pair_ 1 7);
+   Bind (13, Senc) (Encr_ 12 4);
+   Bind (14, Pair) (Pair_ 11 13);
    Send 0 14;
    Return [7]
   ].
