coq/Unilateral.v
@@ -1,36 +1,36 @@
-(** Protocol: unilateral (../rtst/unilateral.scm:5:1) *)
+(** Protocol: unilateral (unilateral.scm:5:1) *)
 
 Require Import Proc.
 Import List.ListNotations.
 Open Scope list_scope.
 Open Scope string.
 
-(** Role: init (../rtst/unilateral.scm:6:3) *)
+(** Role: init (unilateral.scm:6:3) *)
 
 Definition init: proc :=
   mkProc
   [(0, Chan); (1, Akey)]
   [
-   (* Send (../rtst/unilateral.scm:9:7) *)
-   Bind (2, Text) (Nonce);
-   Bind (3, Mesg) (Encr 2 1);
+   (* Send (unilateral.scm:9:7) *)
+   Bind (2, Text) (Nonce_);
+   Bind (3, Aenc) (Encr_ 2 1);
    Send 0 3;
-   (* Recv (../rtst/unilateral.scm:10:7) *)
-   Bind (4, Text) (Recv 0);
+   (* Recv (unilateral.scm:10:7) *)
+   Bind (4, Text) (Recv_ 0);
    Same 4 2;
    Return [2]
   ].
 
-(** Role: resp (../rtst/unilateral.scm:14:3) *)
+(** Role: resp (unilateral.scm:14:3) *)
 
 Definition resp: proc :=
   mkProc
   [(0, Chan); (1, Ikey)]
   [
-   (* Recv (../rtst/unilateral.scm:17:7) *)
-   Bind (2, Mesg) (Recv 0);
-   Bind (3, Text) (Decr 2 1);
-   (* Send (../rtst/unilateral.scm:18:7) *)
+   (* Recv (unilateral.scm:17:7) *)
+   Bind (2, Aenc) (Recv_ 0);
+   Bind (3, Text) (Decr_ 2 1);
+   (* Send (unilateral.scm:18:7) *)
    Send 0 3;
    Return [3]
   ].
